Improve reusability

theories/Reachability/Reachability.v
@@ -1,6 +1,6 @@
 Require Import AllInRel List Map Env DecSolve.
 Require Import IL Annotation AutoIndTac Exp SetOperations.
-Require Export Filter LabelsDefined OUnion.
+Require Export Filter LabelsDefined OUnion WithTop.
 
 Set Implicit Arguments.
 
@@ -31,17 +31,15 @@ Definition isSound (s:sc) :=
 
 Definition uceq (i:sc) (a b:bool) :=
   match i with
-  | Sound => impb a b
-  | Complete => impb b a
-  | SoundAndComplete => a = b
+  | Sound => a -> b
+  | Complete => b -> a
+  | SoundAndComplete => a <-> b
   end.
-
-Hint Extern 0 (uceq _ _ _) => simpl.
 
 Lemma uceq_refl i a
   : uceq i a a.
 Proof.
-  destruct i; simpl; eauto.
+  destruct i; simpl; eauto. reflexivity.
 Qed.
 
 Lemma eq_uceq i (a b:bool)
@@ -56,95 +54,180 @@ Proof.
   intros; subst. eauto using uceq_refl.
 Qed.
 
-Hint Resolve uceq_refl eq_uceq eq_uceq_sym.
+Lemma uceq_trans i (a b c:bool)
+  : uceq i a b -> uceq i b c -> uceq i a c.
+Proof.
+  destruct i; simpl; firstorder.
+Qed.
+
+Hint Resolve uceq_refl.
+
+Hint Immediate eq_uceq_sym eq_uceq.
+
+Lemma uceq_soundandcomplete_sound a b
+  :  uceq SoundAndComplete a b
+     -> uceq Sound a b.
+Proof.
+  simpl; firstorder.
+Qed.
+
+Lemma uceq_soundandcomplete_complete a b
+  :  uceq SoundAndComplete a b
+     -> uceq Complete a b.
+Proof.
+  simpl; firstorder.
+Qed.
+
+Lemma uceq_sound_complete_soundandcomplete a b
+  : uceq Sound a b
+    -> uceq Complete a b
+    -> uceq SoundAndComplete a b.
+Proof.
+  simpl; firstorder.
+Qed.
+
+Hint Immediate uceq_soundandcomplete_sound
+     uceq_soundandcomplete_complete
+     uceq_sound_complete_soundandcomplete.
 
 (** ** The inductive predicate *)
 
-Inductive reachability (i:sc)
+Inductive reachability (ceval:op -> option (withTop bool)) (i:sc)
   : list bool -> stmt -> ann bool -> Prop :=
 | UCPOpr BL x s b e al
-  :  reachability i BL s al
+  :  reachability ceval i BL s al
      -> uceq i b (getAnn al)
-     -> reachability i BL (stmtLet x e s) (ann1 b al)
+     -> reachability ceval i BL (stmtLet x e s) (ann1 b al)
 | UCPIf BL e b1 b2 b al1 al2
-  :  (op2bool e <> Some false -> uceq i b (getAnn al1))
-     -> (op2bool e <> Some true -> uceq i b (getAnn al2))
-     -> reachability i BL b1 al1
-     -> reachability i BL b2 al2
-     -> (if isComplete i then op2bool e = ⎣ false ⎦ -> getAnn al1 = false else True)
-     -> (if isComplete i then op2bool e = ⎣ true ⎦ -> getAnn al2 = false else True)
-     -> reachability i BL (stmtIf e b1 b2) (ann2 b al1 al2)
+  :  (ceval e <> None -> ceval e <> Some (wTA false) -> uceq i b (getAnn al1))
+     -> (ceval e <> None -> ceval e <> Some (wTA true) -> uceq i b (getAnn al2))
+     -> reachability ceval i BL b1 al1
+     -> reachability ceval i BL b2 al2
+     -> (if isComplete i then ceval e = ⎣ wTA false ⎦ -> getAnn al1 = false else True)
+     -> (if isComplete i then ceval e = ⎣ wTA true ⎦ -> getAnn al2 = false else True)
+     -> reachability ceval i BL (stmtIf e b1 b2) (ann2 b al1 al2)
 | UCPGoto BL l Y b a
   : get BL (counted l) b
     -> (if isSound i then impb a b else True)
-    -> reachability i BL (stmtApp l Y) (ann0 a)
+    -> reachability ceval i BL (stmtApp l Y) (ann0 a)
 | UCReturn BL e b
-  : reachability i BL (stmtReturn e) (ann0 b)
+  : reachability ceval i BL (stmtReturn e) (ann0 b)
 | UCLet BL F t b als alt
-  : reachability i (getAnn ⊝ als ++ BL) t alt
+  : reachability ceval i (getAnn ⊝ als ++ BL) t alt
     -> length F = length als
     -> uceq i b (getAnn alt)
     -> (forall n Zs a, get F n Zs ->
                  get als n a ->
-                 reachability i (getAnn ⊝ als ++ BL) (snd Zs) a)
+                 reachability ceval i (getAnn ⊝ als ++ BL) (snd Zs) a)
     -> (if isComplete i then (forall n a,
                                 get als n a ->
                                 getAnn a ->
                                 isCalledFrom (isCalled true) F t (LabI n)) else True)
     -> (if isComplete i then forall n a, get als n a -> impb (getAnn a) b else True)
-    -> reachability i BL (stmtFun F t) (annF b als alt).
+    -> reachability ceval i BL (stmtFun F t) (annF b als alt).
 
+Ltac simpl_isComplete :=
+  match goal with
+  | [ |- context f [ if isComplete Sound then ?A else ?B ] ] =>
+    let x := context f[B] in change x
+  | [ |- context f [ if isComplete Complete then ?A else ?B ] ] =>
+    let x := context f[A] in change x
+  | [ |- context f [ if isComplete SoundAndComplete then ?A else ?B ] ] =>
+    let x := context f[A] in change x
+  | [ H : context f [ if isComplete Sound then ?A else ?B ] |- _ ] =>
+    let x := context f[B] in change x in H
+  | [ H : context f [ if isComplete Complete then ?A else ?B ] |- _ ] =>
+    let x := context f[A] in change x in H
+  | [ H : context f [ if isComplete SoundAndComplete then ?A else ?B ] |- _ ] =>
+    let x := context f[A] in change x in H
+  end.
+
+
+Hint Extern 0 => simpl_isComplete.
 (** ** Some Properties of the Predicate *)
 
-Local Hint Extern 0 =>
-match goal with
-| [ H : op2bool ?e <> Some ?t , H' : op2bool ?e <> Some ?t -> _ |- _ ] =>
-  specialize (H' H); subst
-end.
+Opaque uceq.
 
-Lemma reachability_SC_S Lv s slv
-  : reachability SoundAndComplete Lv s slv
-    -> reachability Sound Lv s slv.
+Lemma reachability_SC_S ceval Lv s slv
+  : reachability ceval SoundAndComplete Lv s slv
+    -> reachability ceval Sound Lv s slv.
 Proof.
   intros UC.
-  general induction UC; simpl in *; subst; eauto 20 using reachability, uceq_refl.
-  - econstructor; simpl; eauto using uceq_refl.
-  - econstructor; simpl; eauto using uceq_refl.
+  general induction UC; subst; eauto 10 using reachability, uceq_soundandcomplete_sound.
 Qed.
 
 Hint Resolve reachability_SC_S.
 
-Lemma reachability_sound_and_complete BL s a
-  : reachability Complete BL s a
-    -> reachability Sound BL s a
-    -> reachability SoundAndComplete BL s a.
+Lemma reachability_sound_and_complete ceval BL s a
+  : reachability ceval Complete BL s a
+    -> reachability ceval Sound BL s a
+    -> reachability ceval SoundAndComplete BL s a.
 Proof.
   intros RCH UCS.
-  general induction UCS; inv RCH; simpl in *; eauto 20 using reachability, impb_eq.
+  general induction UCS; inv RCH; simpl in *;
+    eauto 10 using reachability, uceq_sound_complete_soundandcomplete.
 Qed.
 
+Definition cop2bool e :=
+  match op_eval (fun _ : nat => ⎣⎦) e with
+  | Some v => ⎣ wTA (val2bool v) ⎦
+  | None => Some Top
+  end.
+
+Lemma op2bool_not_none e
+  : cop2bool e <> ⎣⎦.
+Proof.
+  unfold cop2bool; cases; congruence.
+Qed.
+
+Hint Resolve op2bool_not_none.
+
+Lemma op2bool_cop2bool_not_some e b
+  : op2bool e <> ⎣ b ⎦
+    -> cop2bool e <> ⎣ wTA b ⎦.
+Proof.
+  unfold op2bool, cop2bool; intros; cases; simpl in *; congruence.
+Qed.
+
+Transparent uceq.
+
+Ltac std_ind_inst :=
+  match goal with
+    [ H : forall y : stmt, size y < size (stmtLet _ _ ?s) -> _ |- _ ] =>
+    specialize (H s ltac:(eauto))
+  end.
+
+Ltac std_ind_dcr :=
+  match goal with
+  | [ H : forall y : stmt, size y < size (stmtLet _ _ ?s) -> _ |- _ ] =>
+    edestruct (H s ltac:(eauto)); eauto; dcr
+  end.
+
 Lemma reachability_trueIsCalled Lv s slv l
-  : reachability Sound Lv s slv
+  : reachability cop2bool Sound Lv s slv
     -> isCalled true s l
-    -> exists b, get Lv (counted l) b /\ impb (getAnn slv) b.
+    -> exists b, get Lv (counted l) b /\ ((getAnn slv) -> b).
 Proof.
   destruct l; simpl.
   revert Lv slv n.
   sind s; destruct s; intros Lv slv n UC IC; inv UC; inv IC;
-    simpl in *; subst; simpl in *; eauto 20.
-  - edestruct (IH s); dcr; eauto.
-  - edestruct (IH s1); dcr; eauto.
-  - edestruct (IH s2); dcr; eauto.
+    simpl in *; subst; simpl in *; try std_ind_dcr;
+      eauto 20 using op2bool_cop2bool_not_some.
+  - edestruct (IH s1); dcr; eauto 20 using op2bool_cop2bool_not_some.
+  - edestruct (IH s2); dcr; eauto 20 using op2bool_cop2bool_not_some.
+  - eexists; split; eauto. revert H4; clear_all; destruct a; firstorder.
   - destruct l'.
     exploit (IH s); eauto; dcr.
-    setoid_rewrite H3. setoid_rewrite H10.
-    clear H3 H10 UC H9 H1 alt.
-    general induction H5.
-    + inv_get. eexists; split; eauto.
-    + inv_get.
-      exploit H4; eauto.
-      eapply IH in H3; eauto.
-      dcr. inv_get.
-      edestruct IHcallChain; try eapply H8; eauto; dcr.
-      eexists x1; split; eauto.
+    assert ( exists b0 : bool, get Lv n b0 /\ (x -> b0)). {
+      clear H3 H10 UC H9 H1 alt.
+      general induction H5.
+      - inv_get. eexists; split; eauto.
+      - inv_get.
+        exploit H4; eauto.
+        eapply IH in H3; eauto.
+        dcr. inv_get.
+        edestruct IHcallChain; try eapply H8; eauto; dcr.
+        eexists x1; split; eauto.
+    }
+    dcr; eexists; split; eauto.
 Qed.
